examples/map/MapIMproof.v
@@ -33,32 +33,38 @@ Local Open Scope nat_scope.
 
 
 Section SIMMODSEM.
-  Context `{_W: CtxWD.t}.
-  Context `{@GRA.inG MapRA0 Γ}.
+  Context `{_M: MapRA0.t}.
+
+  (* Context `{_W: CtxWD.t}.
+  Context `{@GRA.inG pending0RA Γ}.
+  Context `{@GRA.inG CallableRA Γ}.
+  Context `{@GRA.inG MapStateRA Γ}. *)
+
   Context `{@GRA.inG memRA Γ}. 
-
-  (* Let wf: _ -> W -> Prop :=
-        @inv_wf
-          _ _
-          unit
-          (fun _ st_src st_tgt =>
-             ((∃ blk ofs l (f: Z -> Z) (sz: Z), ⌜st_src = (f, sz)↑ /\ (length l = Z.to_nat sz) /\ (forall k (SZ: (0 <= k < sz)%Z), nth_error l (Z.to_nat k) = Some (f k)) /\ st_tgt = (Vptr blk ofs)↑⌝ ** OwnM ((blk, ofs) |-> (List.map Vint l)) ** pending0) ∨ (⌜st_src = (fun (_: Z) => 0%Z, 0%Z)↑⌝))%I)
-  . *)
-
-
         
   Variable GlobalStbM: Sk.t -> gname -> option fspec.
   Hypothesis STBINCLM: forall sk, stb_incl (to_stb MemStb) (GlobalStbM sk).
+  (* Hypothesis STB_getM: forall sk, (GlobalStbM sk) "get" = Some get_specM. *)
   Hypothesis STB_setM: forall sk, (GlobalStbM sk) "set" = Some set_specM.
 
   Section LEMMA. 
+
+    Lemma callable_unique:
+      callable -∗ callable -∗ False%I.
+    Proof.
+      Local Transparent callable.
+      iIntros "H0 H1". iCombine "H0 H1" as "H".
+      iOwnWf "H". exfalso. clear -H3.
+      rr in H3. ur in H3. unseal "ra". des. ur in H3. ss.
+    Qed.    
+
     Lemma pending0_unique:
       pending0 -∗ pending0 -∗ False%I.
     Proof.
       Local Transparent pending0.
       iIntros "H0 H1". iCombine "H0 H1" as "H".
-      iOwnWf "H". exfalso. clear - H1.
-      rr in H1. ur in H1. unseal "ra". des. ur in H1. ss.
+      iOwnWf "H". exfalso. clear - H3.
+      rr in H3. ur in H3. unseal "ra". des. ur in H3. ss.
     Qed.
 
     Lemma points_to_get_split blk ofs l k v
@@ -96,7 +102,7 @@ Section SIMMODSEM.
       { destruct k; ss; eauto.
         hexploit IHl; eauto.
         { instantiate (1:=k). lia. }
-        i. des. rewrite H1. eauto.
+        i. des. rewrite H3. eauto.
       }
     Qed.
 
@@ -258,7 +264,7 @@ Section SIMMODSEM.
   :
     @isim _ I fls flt r g R RR true pt (st_src, k_src tt) sti_tgt
   -∗  
-    @isim _ I fls flt r g R RR ps pt (st_src, _APC stb at_most o >>= (fun x => tau;; Ret x) >>= k_src) sti_tgt.
+    @isim _ I fls flt r g R RR ps pt (st_src, _APC stb at_most o >>= (fun x => (tau;; Ret x) >>= k_src)) sti_tgt.
   Proof.
     destruct sti_tgt.
     iIntros "K".
@@ -274,10 +280,10 @@ Section SIMMODSEM.
   :
     @isim _ I fls flt r g R RR true pt (st_src, HoareCall true o fsp fn vargs >>= (fun _ => _APC stb next o) >>= (fun x => tau;; Ret x) >>= k_src) sti_tgt
   -∗  
-    @isim _ I fls flt r g R RR ps pt (st_src, _APC stb at_most o >>= (fun x => tau;; Ret x) >>= k_src) sti_tgt.
+    @isim _ I fls flt r g R RR ps pt (st_src, _APC stb at_most o >>= (fun x => (tau;; Ret x) >>= k_src)) sti_tgt.
   Proof.
     destruct sti_tgt.
-    iIntros "K".
+    iIntros "K". prep.
     iEval (rewrite unfold_APC).
     force. instantiate (1:= false). steps.
     force. instantiate (1:= next). unfold guarantee.
@@ -287,42 +293,51 @@ Section SIMMODSEM.
     Unshelve. eauto.
   Qed.
 
-  (* Lemma hcall_clo
+  Lemma hcall_clo
     I fls flt r g ps pt {R} RR st_src st_tgt k_src k_tgt
-    fn vargs o fsp
+    fn varg_src varg_tgt o X (x: shelve__ X) (D: X -> ord) P Q
     (* PURE, ... *)
+    (ORD: ord_lt (D x) o)
+    (PURE: is_pure (D x))
   :
-    (* ((∀st_src0 st_tgt0 vret_src vret_tgt, (I st_src0 st_tgt0) -∗ @isim _ I fls flt r g R RR true pt (st_src0, k_src vret_src) (st_tgt0, k_tgt vret_tgt))) *)
-    (I st_src st_tgt ∗ (∀st_src0 st_tgt0 vret_src vret_tgt, (I st_src0 st_tgt0) -∗ @isim _ I fls flt r g R RR true pt (st_src0, k_src vret_src) (st_tgt0, k_tgt vret_tgt)))
+    (P x varg_src varg_tgt 
+      ∗ I st_src st_tgt 
+      ∗ (∀st_src0 st_tgt0 vret_src vret_tgt, 
+             (Q x vret_src vret_tgt ∗ I st_src0 st_tgt0) 
+          -∗ @isim _ I fls flt r g R RR true true (st_src0, k_src vret_src) (st_tgt0, k_tgt vret_tgt)))
   -∗  
-    @isim _ I fls flt r g R RR ps pt (st_src, HoareCall true o fsp fn vargs >>= k_src) (st_tgt, trigger (Call fn vargs) >>= k_tgt).
+    @isim _ I fls flt r g R RR ps pt (st_src, HoareCall true o (mk_fspec D P Q) fn varg_src >>= k_src) (st_tgt, trigger (Call fn varg_tgt) >>= k_tgt).
   Proof.
-  Admitted. *)
+    iIntros "(P & IST & K)".
+    unfold HoareCall. prep.
+    force. instantiate (1:= x).
+    force. instantiate (1:= varg_tgt).
+    force. iSplitL "P"; [eauto|]. 
+    call; [eauto|].
+    steps. iApply "K". iFrame.
+  Qed.
 
   (****************************)
 
   Local Notation universe := positive.
   (* Local Notation level := nat. *)
 
-  Lemma initialized0_unique k : initialized0 k -∗ initialized0 k -∗ False.
+  (* Lemma initialized0_unique k : initialized0 k -∗ initialized0 k -∗ False.
   Proof. 
     iIntros "I0 I1". iCombine "I0 I1" as "I".
-    iOwnWf "I". clear -H1.
-    rr in H1. ur in H1. unseal "ra". des. ur in H0. ss.
-  Qed.
+    iOwnWf "I". clear -H2.
+    rr in H2. ur in H2. unseal "ra". des. ur in H0. ss.
+  Qed. *)
 
-  Definition init_points blk ofs f k := (initialized0 k ∨ OwnM ((blk, (ofs + k)%Z) |-> [Vint (f k)]))%I.
+  Definition init_points blk ofs f k :=  (OwnM ((blk, (ofs + k)%Z) |-> [Vint (f k)]))%I.
+  (* Definition init_points blk ofs f k := (initialized0 k ∨ OwnM ((blk, (ofs + k)%Z) |-> [Vint (f k)]))%I. *)
 
   Fixpoint mem_index (sz: nat) : list Z :=
       match sz with 0 => [] | S k => (Z.of_nat k) :: mem_index k end.
 
   Definition mem_inv blk ofs f sz := ([∗ list] k ∈ (mem_index sz), init_points blk ofs f k)%I.
 
-  (* Fixpoint mem_inv blk ofs f sz : iProp := 
-    match sz with
-    | 0 => True%I
-    | S sz0 => init_points blk ofs f sz0 ∗ mem_inv blk ofs f sz0
-    end.    *)
+  (* Definition initial_inv := (∀ sz, ([∗ list] k ∈ (mem_index sz), initialized0 k))%I. *)
 
   Lemma mem_inv_split blk ofs f sz k (SZ: 0 <= k < sz): 
     mem_inv blk ofs f sz -∗ (init_points blk ofs f k ∗ (init_points blk ofs f k -* mem_inv blk ofs f sz)).
@@ -340,148 +355,365 @@ Section SIMMODSEM.
     iClear "IH". iDestruct "M" as "[I M]". subst. iFrame. eauto.
   Qed. 
 
+  (* Fixpoint mem_inv_f blk ofs f sz :=
+    match sz with
+    | 0 => True%I
+    | S sz' => (init_points blk ofs f sz' ∗ mem_inv_f blk ofs f sz')%I 
+    end.
+
+  Lemma mem_inv_unfold blk ofs f sz:
+    mem_inv blk ofs f sz -∗ mem_inv_f blk ofs f sz.
+  Proof. 
+    induction sz; ss.
+    iIntros "H". unfold mem_inv. s.
+    iDestruct "H" as "[H0 H1]". iFrame.
+    iApply IHsz. eauto.  
+  Qed. *)
+
+  Lemma mem_inv_split' blk ofs f sz k (SZ: 0 <= k < sz):
+    mem_inv blk ofs f sz -∗ (init_points blk ofs f k ∗ ([∗ list] n ∈ (mem_index sz), if Z.eq_dec n k then True else init_points blk ofs f n)).
+  Proof.
+    induction sz; [lia|].
+    destruct (classic (k = sz)).
+    {
+      subst. iIntros "H". unfold mem_inv. s.
+      iDestruct "H" as "[H0 H1]". iFrame.
+      destruct (Z.eq_dec sz sz); ss. iSplit; eauto.
+      clear IHsz SZ e. generalize sz at 1 5. i.
+      iStopProof. induction sz0; ss.
+      iIntros "[H0 H1]". iSplitL "H0".
+      { des_ifs. }
+      iApply IHsz0. eauto.
+    }
+    iIntros "H". unfold mem_inv. s.
+    iDestruct "H" as "[H0 H1]".
+    destruct (Z.eq_dec sz k); [lia|].
+    iFrame. iApply IHsz; eauto. lia.
+  Qed.
+
+  Definition init_map_st := (fun (_: Z) => 0%Z, 0%Z).
+  
   Let Ist: Any.t -> Any.t -> iProp := 
     (fun st_src st_tgt =>
              ((∃ blk ofs (f: Z -> Z) (sz: Z), 
-             ⌜st_src = (f, sz)↑⌝ 
-             ∗ mem_inv blk ofs f (Z.to_nat sz) ∗ pending0) 
-             ∨ (⌜st_src = (fun (_: Z) => 0%Z, 0%Z)↑⌝))%I).
+                ⌜st_src = (f, sz)↑ /\  st_tgt = (Vptr blk ofs)↑⌝ 
+                ∗ mem_inv blk ofs f (Z.to_nat sz) ∗ pending0 ∗ mapstate_full (init_map_st, Vnullptr)) 
+             ∨ (⌜st_src = init_map_st↑ /\ st_tgt = Vnullptr↑⌝ ∗ mapstate_full (init_map_st, Vnullptr))
+             ∨ (∃ st_src0 st_tgt0, callable ∗ mapstate (st_src0, st_tgt0) ∗ ⌜st_src = st_src0↑ /\ st_tgt = st_tgt0↑⌝))%I).
 
-  (* Let Ist: Any.t -> Any.t -> iProp := 
-    (fun st_src st_tgt =>
-             ((∃ blk ofs (f: Z -> Z) (sz: Z), 
-             ⌜st_src = (f, sz)↑ /\  st_tgt = (Vptr blk ofs)↑⌝ 
-             ∗ mem_inv blk ofs f (Z.to_nat sz) ∗ pending0) 
-             ∨ (⌜st_src = (fun (_: Z) => 0%Z, 0%Z)↑⌝))%I). *)
-
-  (* Let Ist: Any.t -> Any.t -> iProp := 
-    (fun st_src st_tgt =>
-             ((∃ blk ofs (f: Z -> Z) (sz: Z), 
-             ⌜st_src = (f, sz)↑ /\  st_tgt = (Vptr blk ofs)↑⌝ 
-             ∗ (∀ k (SZ: (0 <= k < sz)%Z), initialized0 k ∨ OwnM ((blk, (ofs + k)%Z) |-> [Vint (f k)])) ∗ pending0) 
-             ∨ (⌜st_src = (fun (_: Z) => 0%Z, 0%Z)↑⌝))%I). *)
-            
   Theorem sim: HModPair.sim (MapM.HMap GlobalStbM) (MapI.Map) Ist.
   Proof.
-    econs; eauto; ii; econs; cycle 1; [s|sim_split].
-    - iIntros "_". iSplitR; eauto. 
-      steps. iRight. iFrame. esplits; eauto.
+    sim_init.
+    - iIntros "H". iSplitR; eauto. 
+      steps. iRight. iLeft. iFrame. esplits; eauto.
     - unfold cfunU, initF, MapI.initF, interp_sb_hp, HoareFun, ccallU. s.
-      steps. iDestruct "ASM" as "(W & (%Y & %M & P0) & %X)". subst.
-      iDestruct "IST" as "[IST|%]".
+      steps. iDestruct "ASM" as "(W & (%Y & %M & P0 & C) & %X)". subst.
+      iDestruct "IST" as "[IST|[IST|IST]]"; swap 2 3.
       {
-        iDestruct "IST" as (? ? ? ?) "(_ & _ & P)".
+        iDestruct "IST" as (? ? ? ?) "(_ & _ & P & M)".
         iExFalso. iApply (pending0_unique with "P P0").
       }
+      {
+        iDestruct "IST" as (? ?) "(C0 & _)".
+        iExFalso. iApply (callable_unique with "C C0"). 
+      }
+      iDestruct "IST" as "[% M]".
       rewrite Any.upcast_downcast in G. inv G. simpl in G0. inv G0.
-      (* des. subst.  *)
-      steps. 
-      iApply APC_start_clo. instantiate (1:= 1 + x).
-      iApply APC_step_clo.
+      des. subst. 
+      steps.
+      iApply APC_start_clo. instantiate (1:= 1 + x). prep. iApply APC_step_clo.
       { eapply STBINCLM. instantiate (2:= "alloc"). stb_tac. ss.  }
       { eapply OrdArith.lt_from_nat. eapply Nat.lt_succ_diag_r. }
-
-      (*** TODO: Make a lemma for < HoareCall / Call >***)
       instantiate (1:= Any.upcast [Vint x]).
       rewrite HoareCall_parse. prep. 
       unfold HoareCallPre. steps.
       force. instantiate (1:= x). 
       force. instantiate (1:= Any.upcast [Vint x]). 
       force. iSplitR; [eauto|].
-      iRename "P0" into "IST". call.
-      {   
-        iLeft. iExists _, _, (λ _ : Z, 0%Z), x.
-        iFrame. iSplit.
-        { 
-          iPureIntro. esplits; eauto.
-          admit.
-        }
-        admit. 
-      } 
-      unfold HoareCallPost.
-      steps.
+      iPoseProof (mapstate_update with "M") as "M".
+      iMod "M". instantiate (1:= (((λ _ : Z, 0%Z), Z.of_nat x), Vnullptr)).
+      iDestruct "M" as "[MB MW]".
+      iCombine "C MW" as "IST". call.
+      { 
+        iRight. iRight. 
+        iExists ((λ _ : Z, 0%Z), Z.of_nat x), Vnullptr. 
+        iDestruct "IST" as "[C M]". iFrame. eauto. 
+      }
+      iDestruct "IST" as "[IST|[IST|IST]]".
+      {
+        iDestruct "IST" as (? ? ? ?) "(_ & _ & P & _)".
+        iExFalso. iApply (pending0_unique with "P P0").
+      }
+      {
+        iDestruct "IST" as "[% [MB0 MW]]". 
+        iExFalso. iApply (mapstate_auth_unique with "MB MB0").  
+      }
+      iDestruct "IST" as (? ?) "[C [MW %]]".
+      iPoseProof (mapstate_eq with "MB MW") as "%".
+      des. subst. inv H4.
+      unfold HoareCallPost. steps.
       iDestruct "ASM" as "[ASM %]".
       iDestruct "ASM" as ( ? ) "[% ASM]". subst.
-      (* iPoseProof () *)
       steps. 
-      admit.
+      pattern 0%Z at 10.
+      match goal with
+      | |- ?P 0%Z => cut (P (x-x)%Z)
+      end; ss.
+      { rewrite Z.sub_diag. ss. }
+      assert (OwnM ((b, 0%Z) |-> repeat Vundef x) -∗ OwnM ((b, 0%Z) |-> (repeat (Vint 0) (x - x) ++ repeat Vundef x))).
+      { iIntros "H". rewrite Nat.sub_diag. ss. }
+      iPoseProof (H3 with "ASM") as "O".
+      iStopProof.
+      cut (x <= x); [|lia].
+      generalize x at 1 6 7 9 14. intros n. induction n; i; iIntros "(W & P0 & MB & C & MW & O)".
+      { 
+        rewrite unfold_iter. 
+        steps. des_ifs; [lia|].
+        iApply APC_stop_clo. steps. 
+        force. force.
+        iSplitL "W C". { iFrame. eauto. }
+        iPoseProof (mapstate_update with "[MB MW]") as ">M"; [iFrame|].
+        instantiate (1:= (init_map_st, Vnullptr)).
+        steps. iSplit; [|eauto].
+        iLeft. iExists _, _, _, _.
+        iFrame. iSplit; eauto.
+        replace (Z.to_nat x) with (x - 0); [|lia].
+        rewrite app_nil_r.
+        unfold mem_inv, init_points.
+        replace (x - 0) with x; [|lia].
+        iStopProof. induction x; eauto.
+        iIntros "O"; s. 
+        rewrite repeat_cons. rewrite points_to_app.
+        iDestruct "O" as "[H0 H1]". rewrite repeat_length. iFrame.
+        iApply IHx; [lia| |lia|lia|eauto].
+        replace (x-x) with 0; [|lia].
+        iIntros "H". rewrite points_to_app. rewrite repeat_length. s.
+        rewrite points_to_nil. r_solve. 
+        replace (0 + 0)%Z with 0%Z; [eauto|lia].
+      }
+      {
+        rewrite unfold_iter. steps. des_ifs.
+        2: { exfalso. lia. }
+        steps. unfold scale_int at 1. des_ifs.
+        2: { exfalso. eapply n0. eapply Z.divide_factor_r. }
+        steps.
+        assert (EQ: (0 + ((x - S n)%nat * 8) `div` 8) = (x - S n)).
+        { rewrite Nat.div_mul; ss. }
+        assert (
+        OwnM ((b, 0%Z) |-> (repeat (Vint 0) (x - S n) ++ Vundef :: repeat Vundef n))
+        -∗
+        (OwnM ((b, Z.of_nat (x - S n)) |-> [Vundef]) ** (OwnM ((b, Z.of_nat (x - S n)) |-> [Vint 0]) -* OwnM ((b, 0%Z) |-> (repeat (Vint 0) (x - n) ++ repeat Vundef n))))
+        ).
+        { 
+          iIntros "H". rewrite points_to_app. rewrite points_to_split.
+          iDestruct "H" as "[H0 [H1 H2]]". iSplitL "H1".
+          {
+            replace (x - S n: Z) with (0 + strings.length (repeat (Vint 0) (x - S n)))%Z; ss.
+            rewrite repeat_length. lia.
+          }
+          iIntros "H1". rewrite points_to_app.
+          remember ((b, 0%Z) |-> repeat (Vint 0) (x - n)).
+          remember ((b, (0 + length (repeat (Vint 0) (x - n)))%Z) |-> repeat Vundef n).
+          assert (OwnM c ∗ OwnM c0 -∗ OwnM (c ⋅ c0)).
+          { iIntros "[H0 H1]". iCombine "H0 H1" as "H". eauto. }
+          subst. iApply H5.
+          iSplitL "H0 H1".
+          {
+            assert (LEN: x - S n = length (repeat (Vint 0) (x - S n))%Z).
+            { rewrite repeat_length. refl. }
+            iEval (rewrite LEN) in "H1".
+            iCombine "H0 H1" as "H". iEval (rewrite <- points_to_app) in "H".
+            replace (repeat (Vint 0) (x - S n) ++ [Vint 0]) with (repeat (Vint 0) ((x - S n) + 1)).
+            { replace (x - S n + 1) with (x - n); ss. lia. }
+            { rewrite repeat_app; ss. }
+          }
+          replace (0 + strings.length (repeat (Vint 0) (x - n)))%Z with
+          (0 + strings.length (repeat (Vint 0) (x - S n)) + 1)%Z; ss.
+          repeat rewrite repeat_length. rewrite <- Z.add_assoc. lia.
+        }
+        iPoseProof (H5 with "O") as "[H0 H1]".
+        iApply APC_step_clo.
+        { eapply STBINCLM. instantiate (2:= "store"). stb_tac. ss. }
+        { eapply OrdArith.lt_from_nat. instantiate (1:=n). lia. }
+        instantiate (1:= (Any.upcast [Vptr b (0 + ((x - Z.pos (Pos.of_succ_nat n)) * 8) `div` 8); Vint 0])).
+        rewrite HoareCall_parse. prep.
+        unfold HoareCallPre.
+        force. Unshelve. 2: { eapply (b, (x - S n)%Z, Vint 0). }
+        force. Unshelve. 2: { eapply ([Vptr b (0 + ((x - Z.pos (Pos.of_succ_nat n)) * 8) `div` 8); Vint 0]↑). }
+        force. iSplitL "H0". 
+        { 
+          iSplit; eauto. iSplit; eauto. 
+          iExists Vundef. iSplitR.
+          { 
+            iPureIntro. 
+            replace (0 + ((x - Z.pos (Pos.of_succ_nat n)) * 8) `div` 8)%Z with (x - Z.pos (Pos.of_succ_nat n))%Z; eauto. 
+            rewrite Z.div_mul; lia.
+          }
+          replace (x - Z.pos (Pos.of_succ_nat n))%Z with (Z.of_nat (Init.Nat.sub x (S n))); [eauto|lia].
+        }
+        steps. iCombine "MB MW" as "M". 
+        iPoseProof (mapstate_update with "M") as ">[MB MW]". instantiate (1:= ((λ _ : Z, 0%Z, Z.of_nat x), Vptr b 0)).
+        iCombine "C MW" as "IST".
+        call.
+        { 
+          iRight. iRight. iDestruct "IST" as "[C MW]".
+          iExists _, _. iFrame. eauto.
+        }
+        iDestruct "IST" as "[IST|[IST|IST]]".
+        { 
+          iDestruct "IST" as (? ? ? ?) "(_ & _ & P & _)".  
+          iExFalso. iApply (pending0_unique with "P P0").
+        }
+        {
+          iDestruct "IST" as "[_ [MB0 _]]".
+          iExFalso. iApply (mapstate_auth_unique with "MB MB0").  
+        }
+        iDestruct "IST" as (? ?) "(C & MW & %)".
+        iPoseProof (mapstate_eq with "MB MW") as "%".
+        des. inv H7.    
+        unfold HoareCallPost. steps.
+        iDestruct "ASM" as "[ASM %]".
+        iDestruct "ASM" as "[H0 %]". subst.
+        steps. 
+        replace (x - Z.pos (Pos.of_succ_nat n) + 1)%Z with (x - n)%Z; [|lia].
+        replace (x - Z.pos (Pos.of_succ_nat n))%Z with (Z.of_nat (Init.Nat.sub x (S n))); [|lia].
+        iPoseProof ("H1" with "H0") as "O". 
+        iPoseProof (mapstate_update with "[MB MW]") as ">[MB MW]";[iFrame|].
+        instantiate (1:= (λ _ : Z, 0%Z, Z.of_nat x, Vnullptr)).
+        iApply IHn; [lia|iFrame].
+      }
 
     - unfold cfunU, getF, MapI.getF, interp_sb_hp, HoareFun, ccallU. s.
       steps. iDestruct "ASM" as "(W & (% & INIT) & %)". subst. 
       rewrite Any.upcast_downcast in *. steps.
-      iDestruct "IST" as "[IST|%]"; cycle 1.
-      { des. subst. steps. exfalso. lia. }
-      iDestruct "IST" as (? ? ? ?) "(% & MAP & P0)".
+      iDestruct "IST" as "[IST|[IST|IST]]"; swap 1 3.
+      { 
+        iDestruct "IST" as (? ?) "[C _]". 
+        iExFalso. iApply (callable_unique with "C INIT").
+      }
+      {
+        iDestruct "IST" as "[% _]".
+        des. subst. steps. exfalso. lia. 
+      }
+      iDestruct "IST" as (? ? ? ?) "(% & MEM & P0 & M)".
       des. subst. steps. 
       unfold scale_int. des_ifs; cycle 1.
       { exfalso. eapply n. eapply Z.divide_factor_r. }
       steps. iApply APC_start_clo. instantiate (1:= 1).
-      iApply APC_step_clo.
+      prep. iApply APC_step_clo.
       { eapply STBINCLM. instantiate (2:= "load"). stb_tac. ss. }
       { eapply OrdArith.lt_from_nat. eapply Nat.lt_succ_diag_r. } 
       symmetry in G0. inv G0.
       replace (ofs + (x * 8) `div` 8)%Z with (ofs + Z.to_nat x)%Z. 
       2: { rewrite Z_div_mult; ss. lia. }
       instantiate (1:= (Any.upcast [Vptr blk (ofs + Z.to_nat x)])).
-      iPoseProof (mem_inv_split with "MAP") as "[IP MAP]".
+      iPoseProof (mem_inv_split with "MEM") as "[IP MEM]".
       { instantiate (1:= Z.to_nat x). lia. }
-
       prep. unfold HoareCall.
       force. instantiate (1:= (blk, (ofs + Z.to_nat x)%Z, _)).
       force. force.
-      iDestruct "IP" as "[INIT'|POINT]".
-      { 
-        iExFalso. iApply (initialized0_unique with "INIT").
-        iEval (rewrite ZifyInst.of_nat_to_nat_eq) in "INIT'".
-        inv G1. replace (Z.max 0 x) with x. 2: { destruct x; eauto. lia. }
-        eauto.
-      } 
-      iSplitL "POINT".
+      iSplitL "IP".
       { 
         iFrame. repeat iSplit; eauto.
-      } 
-      iCombine "P0 INIT MAP" as "IST".
+      }
+      iPoseProof (mapstate_update with "M") as ">[MB MW]".
+      instantiate (1:= (f, sz, Vptr blk ofs)).
+      iCombine "INIT MW" as "IST".
       call.
       {
-        iDestruct "IST" as "(P0 & INIT & MAP)".
-        iLeft. iExists blk, ofs, f ,sz. iFrame.
-        repeat iSplit; eauto.
-        iApply "MAP". iLeft.  
-        iEval (rewrite ZifyInst.of_nat_to_nat_eq).
-        inv G1. replace (Z.max 0 x) with x. 2: { destruct x; eauto. lia. }
-        eauto.
+        iRight. iRight. iDestruct "IST" as "[C MW]".
+        iExists (f, sz), (Vptr blk ofs). iFrame.
+        iSplit; eauto.
       }
+      iDestruct "IST" as "[IST|[IST|IST]]".
+      {
+        iDestruct "IST" as (? ? ? ?) "(_ & _ & P & _)".
+        iExFalso. iApply (pending0_unique with "P P0").
+      }
+      {
+        iDestruct "IST" as "[_ [MB0 _]]".
+        iExFalso. iApply (mapstate_auth_unique with "MB MB0"). 
+      }
+      iDestruct "IST" as (? ?) "(C & MW & %)".
+      iPoseProof (mapstate_eq with "MB MW") as "%". 
+      des. inv H4.
       steps. 
       rewrite unfold_APC. 
       force. instantiate (1:= true). steps. 
       force. instantiate (1:= vret).
       iDestruct "ASM" as "[[A %] %]". subst.
       steps. force.
-      iSplitR "IST".
-      { 
-        iFrame. 
-        iSplit.
-        { admit. }
-        { iPureIntro. do 3 f_equal. lia. }  
-      }
-      (* instantiate (1:= Vint (f y3)). steps. *)
-      steps. eauto.
+      iSplitL "W C".
+      { iFrame. iPureIntro. do 3 f_equal. lia. }
+      iCombine "MB MW" as "M". iPoseProof (mapstate_update with "M") as ">M".
+      instantiate (1:= (init_map_st, Vnullptr)).
+      steps. iSplitL; eauto. iLeft. iFrame.
+      iExists blk, ofs, f, sz. iSplit; eauto.
+      iApply "MEM". unfold init_points. eauto.
     
     - unfold cfunU, setF, MapI.setF, interp_sb_hp, HoareFun, ccallU. s.
-      steps. destruct y0. iDestruct "ASM" as "%". des_ifs.
-      iDestruct "IST" as "[IST|%]"; cycle 1.
-      { subst. steps. exfalso. lia. }
-      iDestruct "IST" as (? ? ? ? ?) "(% & MAP & P0)".
-      des. subst.
-      rewrite G. steps.
-      rewrite Heq. rewrite Heq0. steps.
+      steps. iDestruct "ASM" as "(W & (% & INIT) & %)". subst. 
+      rewrite Any.upcast_downcast in *. steps.
+      iDestruct "IST" as "[IST|[IST|IST]]"; swap 1 3.
+      { 
+        iDestruct "IST" as (? ?) "[C _]". 
+        iExFalso. iApply (callable_unique with "C INIT").
+      }
+      {
+        iDestruct "IST" as "[% _]".
+        des. subst. steps. exfalso. lia. 
+      }
+      iDestruct "IST" as (? ? ? ?) "(% & MEM & P0 & M)".
+      des. subst. steps. 
       unfold scale_int. des_ifs; cycle 1.
-      { exfalso. eapply n0. eapply Z.divide_factor_r. }
+      { exfalso. eapply n. eapply Z.divide_factor_r. }
       steps. iApply APC_start_clo. instantiate (1:= 1).
-      iApply APC_step_clo.
+      prep. iApply APC_step_clo.
       { eapply STBINCLM. instantiate (2:= "store"). stb_tac. ss. }
       { eapply OrdArith.lt_from_nat. eapply Nat.lt_succ_diag_r. }
-      instantiate (1:= Any.upcast [Vptr blk (ofs + (y4 * 8) `div` 8); Vint y5]).
+      instantiate (1:= Any.upcast [Vptr blk (ofs + (x0 * 8) `div` 8); Vint x1]).
+      symmetry in Heq, Heq0. inv Heq. inv Heq0.
+      replace (ofs + (x0 * 8) `div` 8)%Z with (ofs + Z.to_nat x0)%Z. 
+      2: { rewrite Z_div_mult; ss. lia. }
+      iPoseProof (mem_inv_split with "MEM") as "[IP MEM]".
+      { instantiate (1:= Z.to_nat x0). lia. }
+      unfold HoareCall.
+      force. instantiate (1:= (blk, (ofs + Z.to_nat x0)%Z, _)).
+      force. force. iSplitL "IP".
+      { iSplit; eauto. }
+      iPoseProof (mapstate_update with "M") as ">[MB MW]".
+      instantiate (1:= ((λ n : Z, if Z.eq_dec n x0 then x1 else f n, sz), (Vptr blk ofs))).
+      iCombine "INIT MW" as "IST". call.
+      {
+        iRight. iRight. iDestruct "IST" as "[C MW]". 
+        iExists _, _. iFrame. iSplit; eauto.
+      }
+      iDestruct "IST" as "[IST|[IST|IST]]".
+      {
+        iDestruct "IST" as (? ? ? ?) "(_ & _ & P & _)".
+        iExFalso. iApply (pending0_unique with "P P0"). 
+      }
+      {
+        iDestruct "IST" as "[_ [MB0 _]]".
+        iExFalso. iApply (mapstate_auth_unique with "MB MB0").
+      }
+      iDestruct "IST" as (? ?) "[C [MW %]]".
+      iPoseProof (mapstate_eq with "MB MW") as "%".
+      des. inv H4.
+      steps. iDestruct "ASM" as "[[A %] %]". subst.
+      iApply APC_stop_clo. steps.
+      force. force.
+      iSplitL "W C". { iFrame. eauto. }
+      iCombine "MB MW" as "M". iPoseProof (mapstate_update with "M") as ">M".
+      instantiate (1:= (init_map_st, Vnullptr)).
+      steps. iSplitL; eauto. iLeft. iExists _, _, _, _.
+      iSplit; eauto. iFrame.
+      (***********************************)
+
+
+
+
+
       hexploit set_nth_success.
       { rewrite H2. instantiate (1:= Z.to_nat y4). lia. }
       i. des.
